Work on validator, esp binary ops.

Validator.v
@@ -1,197 +1,283 @@
+Add LoadPath "~/Downloads/htt/v8.2".
 Require Import Equations.
+Require Import CSDL.Binary.
+Obligation Tactic := program_simpl.
 
 Equations(nocomp) nth_prf {A} (n : nat) (l : list A) (p : n < length l) : A :=
 nth_prf A n nil pf :=! pf;
 nth_prf A O (cons a l) pf := a ;
 nth_prf A (S n) (cons a l) pf := nth_prf n l _.
 
-  Next Obligation. inversion pf. Defined.
   Next Obligation. auto with arith. Defined.
-  Next Obligation. find_empty. Defined.
+
+Equations(nocomp) bits_enum (n : nat) : list (bits n) :=
+bits_enum 0 := [ Vnil] ;
+bits_enum (S n) := let bn := bits_enum n in
+  map (Vcons true) bn ++ map (Vcons false) bn.
 
 Require Import Asm.X86.X86.
 Require Import Asm.Bitvector.Bitvector.
 Require Import String.
 Require Import Bvector.
-Require Import CSDL.Vector.
-Require Import CSDL.Binary.
 Require Import CSDL.Representable.
 Require Import CSDL.BinaryBe.
 
+Require Import CSDL.EqDec_instr.
+
 Definition regset := Int32Map.t bool.
 
-Definition instr_is_disallowed (i : instr) :=
-  match i with
-    (* Disallow [ret] and indirect calls through memory. *)
-    | Ret => true
-    | Call op | Jmp op =>
-      match op with
-        | Address _ => true
-        | _ => false
-      end
-    | _ => false
-  end.
+(* Disallow [ret] and indirect calls through memory. *)
+
+Equations(nocomp) instr_is_disallowed (i : instr) : bool :=
+instr_is_disallowed Ret := true ;
+instr_is_disallowed (Call (Address _)) := true ;
+instr_is_disallowed (Jmp (Address _)) := true ;
+instr_is_disallowed _ := false.
 
 Require Import CSDL.Hexadecimal.
 Require Import CSDL.Show.
 
-Definition cs_mask : bits 32 :=
-  fst (binary_minus_be full (representation 32 31)).
+Definition block_size := 32. (* bytes *)
 
-Eval vm_compute in (eq_refl : print cs_mask = "0xffffffe0")%string.
+Definition binary_shiftl_n_full {n} (b : bits n) m : bits (n + m) :=
+  vector_append b zero.
+
+Definition block_size_mask : bits 32 :=
+  binary_shiftl_n_full (@full 27) 5.
+
+Definition block_offset_mask := 
+  binary_inverse block_size_mask.
+
+Fact block_size_mask_hex : print block_size_mask = "0xffffffe0"%string.
+Proof. reflexivity. Qed.
 
 Definition nacl_jmp_instr : (instr * instr) :=
-  (Arith And (Reg EAX) (Imm _ cs_mask), Jmp (Reg EAX)).
-
-Require Import EquivDec.
-
-Instance: EqDec int32 eq.
-Proof. apply const_eq. Defined.
-
-Ltac dec_eq_one := 
-  match goal with 
-    | H : ?x =/= ?x |- _ => elimtype False; apply H; reflexivity
-    | H : ?x === ?y |- _ => red in H; subst
-    | |- { ?x === ?x } + { _ } => left; reflexivity
-    | |- { _ } + { ?x =/= ?x } => left; f_equal
-    | |- { ?x === ?y } + { _ } => right; let H := fresh in intro H; red in H; 
-      (injection H || discriminate); intros; subst
-  end.
-
-Ltac dec_eq := try solve [ repeat dec_eq_one ];
-  repeat match goal with H : _ === _ |- _ => red in H; subst end.
-
-Instance option_eq_dec {A} `(EqDec A eq) : EqDec (option A) eq.
-Proof.
-  intros x y. destruct x; destruct y; dec_eq.
-  destruct (equiv_dec a a0); dec_eq. 
-Qed.
-
-Instance reg32_eq_dec : EqDec reg32 eq.
-  intros x y. apply reg32_eq_dec. 
-Qed.
-
-Instance reg8_eq_dec : EqDec reg8 eq.
-  intros x y. change ({x = y} + {x <> y}).
-  decide equality x y. 
-Qed.
-
-Instance scale_eq_dec : EqDec scale eq.
-  intros x y. change ({x = y} + {x <> y}). 
-  decide equality x y.
-Qed.
-
-Instance: EqDec address eq. 
-  red; intros. destruct x; destruct y; dec_eq.
-  destruct (equiv_dec addrDisp addrDisp0); dec_eq.
-  destruct (equiv_dec addrBase addrBase0); dec_eq.
-  destruct (equiv_dec addrIndex addrIndex0); dec_eq.
-Qed.
-
-Instance genop_eq_dec : EqDec genop32 eq.
-  intros x y. change ({x = y} + {x <> y}).
-  decide equality x y. 
-  apply int32_eq_dec. apply reg32_eq_dec. 
-  apply equiv_dec.
-Qed.
-
-Instance genop8_eq_dec : EqDec genop8 eq.
-  intros x y. change ({x = y} + {x <> y}).
-  decide equality x y. 
-  apply int32_eq_dec. apply reg8_eq_dec. 
-  apply equiv_dec.
-Qed.
-
-Instance arith_op_eq_dec : EqDec arith_op eq.
-  intros x y. change ({x = y} + {x <> y}).
-  decide equality x y. 
-Qed.
-
-Instance condition_eq_dec : EqDec condition eq.
-  intros x y. change ({x = y} + {x <> y}).
-  decide equality x y. 
-Defined.
-
-Instance cc_eq_dec : EqDec cc eq.
-  intros x y. change ({x = y} + {x <> y}).
-  decide equality x y. 
-  apply condition_eq_dec.
-  apply equiv_dec.
-Qed.
-
-Instance shift_op_eq_dec : EqDec shift_op eq.
-  intros x y. change ({x = y} + {x <> y}).
-  decide equality x y. 
-Qed.
-
-Instance instr_eq_dec : EqDec instr eq.
-  intros x y. 
-  destruct x; destruct y; dec_eq.
-  Ltac add_eq :=
-    match goal with
-      | [ x : ?T, y : ?T |- _ ] =>
-        match goal with 
-          | H : x === y |- _ => red in H; subst
-          | _ => destruct (equiv_dec x y)
-        end
-    end. 
-  destruct (equiv_dec a a0); dec_eq.
-  destruct (equiv_dec g g1); dec_eq.
-  destruct (equiv_dec g0 g2); dec_eq.
-
-  destruct (equiv_dec a a0); dec_eq.
-  destruct (equiv_dec g g1); dec_eq.
-  destruct (equiv_dec g0 g2); dec_eq.
-
-  destruct (equiv_dec g g0); dec_eq.
-
-  destruct (equiv_dec g g1); dec_eq.
-  destruct (equiv_dec g0 g2); dec_eq.
-
-  destruct (equiv_dec g g0); dec_eq.
-
-  destruct (equiv_dec i i0); dec_eq.
-  destruct (equiv_dec c c0); dec_eq.
-
-  destruct (equiv_dec g g0); dec_eq.
-
-  destruct (equiv_dec r r0); dec_eq.
-  destruct (equiv_dec a a0); dec_eq.
-
-  destruct (equiv_dec g g1); dec_eq.
-  destruct (equiv_dec g0 g2); dec_eq.
-
-  destruct (equiv_dec g g1); dec_eq.
-  destruct (equiv_dec g0 g2); dec_eq.
-
-  destruct (equiv_dec g g0); dec_eq.
-
-  destruct (equiv_dec g g0); dec_eq.
-
-  destruct (equiv_dec s s0); dec_eq.
-  destruct (equiv_dec g g1); dec_eq.
-  destruct (equiv_dec g0 g2); dec_eq.
-Defined.
+  (Arith And (Reg EAX) (Imm _ block_size_mask), Jmp (Reg EAX)).
 
 Definition is_nacl_jmp_idiom i j :=
   let '(a, b) := nacl_jmp_instr in
     equiv_decb a i && equiv_decb b j.
 
-Definition block_size := 32. (* bytes *)
-Definition block_size_bin : bits 32 := 
-  representation (e:=BigEndian) 32 32.
-Definition block_size_mask : bits 32 :=
-  binary_shiftl_n_full full 5.
+(** 32 byte block of an instruction. *)
 
 Definition block (ip : int32) : int32 :=
-  BVand 32 ip (vector_append (full (n:=30)) (zero (n:=2))).
+  BVand 32 ip block_size_mask.
+
+Definition block_offset (ip : int32) : int32 :=
+  BVand 32 ip block_offset_mask.
 
 Parameter decode_instr : int32 -> instr * int32.
 Parameter instr_length : int32 -> int32.
 
-Definition instr_overlaps_block_size (ip : int32) : bool :=
-  let (instrend, of) := binary_plus_be ip (instr_length ip) in
-    of || negb (binary_eq zero (BVand 32 block_size_mask instrend)).
+Equations(nocomp) instr_overlaps_block_size (ip : int32) : bool :=
+instr_overlaps_block_size ip
+  with binary_plus_be (block_offset ip) (instr_length ip) :=
+  | pair offset of := negb (binary_eq (block offset) zero).
+
+Ltac destruct_bits :=
+  repeat match goal with
+           | b : bit |- _ => destruct b 
+           | b : bool |- _ => destruct b 
+         end.
+
+Class Commutative {A B} (f : A -> A -> B) := commutative : Π x y, f x y = f y x.
+
+Instance andb_comm : Commutative andb := andb_comm.
+Instance orb_comm : Commutative orb := orb_comm.
+Instance xorb_comm : Commutative xorb := xorb_comm.
+
+Instance Vbinary_comm {f} `(Commutative bool bool f) n : 
+  Commutative (Vbinary bool f n).
+Proof. intros x y. induction n. simpl. reflexivity.
+  depelim x; depelim y.
+  simpl. rewrite (commutative (f:=f)), IHn. reflexivity.
+Qed.
+
+Lemma BVand_mask_zero (x : bits 32) : block x = zero -> [: x] <= pow_of_2 5.
+Proof. intros. unfold block in H. Transparent BVand.
+  unfold BVand in H.
+  repeat depelim x.
+  unfold block_size_mask, zero in H.
+  rewrite (commutative (f:=Vbinary bool andb 32)) in H.
+  simpl in H.
+  injection H. clear H; intros; subst.
+  change (pow_of_2 5) with 32.
+  apply leb_complete. destruct_bits; reflexivity.
+Qed.
+
+Notation " f $ x " := (f x) (only parsing, at level 10, x at level 60).
+
+Class Absorbant {A} (f : A -> A -> A) (a : A) := absorbant : forall x, f a x = a.
+Class Neutral {A} (f : A -> A -> A) (a : A) := neutral : forall x, f a x = x.
+
+Ltac crush := 
+  try red; intros; destruct_bits; firstorder.
+
+Instance andb_absorbant : Absorbant andb false.
+Proof. crush. Qed.
+
+Instance andb_neutral : Neutral andb true.
+Proof. crush. Qed.
+
+Instance orb_absorbant : Absorbant orb true.
+Proof. crush. Qed.
+
+Instance orb_neutral : Neutral orb false.
+Proof. crush. Qed.
+
+Instance Vbinary_absorbant `(Absorbant bool f a) n : Absorbant (Vbinary bool f n) (constant_vector n a).
+Proof. intros v. induction v. reflexivity.
+  simpl. rewrite IHv. rewrite (absorbant a0). reflexivity.
+Qed.
+
+Instance Vbinary_neutral `(Neutral bool f a) n : Neutral (Vbinary bool f n) (constant_vector n a).
+Proof. intros v. induction v. reflexivity.
+  simpl. rewrite IHv. rewrite (neutral a0). reflexivity.
+Qed.
+
+Definition next_ip (ip : int32) : int32 :=
+  fst $ binary_plus_be ip (instr_length ip).
+
+Parameter text_limit : int32.
+
+Parameter ip_length : forall ip, binary_be_lt ip text_limit = true ->
+  binary_be_le (next_ip ip) text_limit = true.
+
+Lemma BVand_shiftl_full n k (x : bits (n + k)) : 
+  BVand _ x (binary_shiftl_n_full (@full n) k) = 
+  vector_append (fst (vector_split x)) zero.
+Proof.
+  funelim (vector_split x). Transparent BVand. unfold binary_shiftl_n_full.
+  simp vector_append. induction x; simpl; auto.
+  rewrite (commutative (f:=andb)). rewrite (absorbant (f:=andb)). 
+  fold (@zero n).
+  rewrite IHx. reflexivity.
+  destruct (vector_split v).
+  simpl in *. f_equal.
+  rewrite (commutative (f:=andb)). rewrite (neutral (f:=andb)). reflexivity.
+  rewrite <- H.
+  f_equal.
+Qed.
+
+Definition un_of {n} (r : bits n * overflow) : bits n := fst r.
+Typeclasses Transparent BVand.
+
+Require Import CSDL.Basics.
+Require Import Numbers.Natural.Peano.NPeano.
+Import Nat.
+
+Lemma Vbinary_nil (f : bool -> bool -> bool) :
+  Vbinary bool f _ Vnil Vnil = Vnil.
+Proof.
+  simpl. reflexivity.
+Qed.
+
+Lemma Vbinary_cons (f : bool -> bool -> bool) n (a b : bool) (x y : bits n) : 
+  Vbinary bool f (Datatypes.S n) (a |:| x)%vect (b |:| y)%vect = (f a b |:| Vbinary bool f n x y)%vect.
+Proof.
+  simpl. reflexivity.
+Qed.
+
+Opaque Vbinary.
+Hint Rewrite Vbinary_nil Vbinary_cons : Vbinary.
+
+Lemma BVxor_absorbant n (x : bits n) : BVxor n (constant_vector n true) x = binary_inverse x.
+Proof.
+  induction x; simp binary. simpl. rewrite IHx. reflexivity.
+Qed.
+
+Lemma BVxor_neutral n (x : bits n) : BVxor n (constant_vector n false) x = x.
+Proof.
+  induction x; simp binary. simpl. rewrite IHx. destruct a; reflexivity.
+Qed.
+
+Lemma nat_of_vector_split {n k} (x : bits (n + k)) : 
+  let (high, low) := vector_split x in
+    [: x ] = pow_of_2 k * [: high ] + [: low ].
+Proof.
+  funelim (vector_split x).
+  omega.
+  destruct (vector_split v). destruct a.
+  simpl. rewrite H. simp pow_of_2. ring.
+
+  rewrite H.
+  simpl. auto.
+Qed.
+
+Lemma modulo_nat_binary {n k} (x : bits (n + k)) : 
+  modulo [: x ] (pow_of_2 k) = [: snd (vector_split x) ].
+Proof.
+  assert (splitx := nat_of_vector_split x). destruct (vector_split x).
+  rewrite splitx.
+  simpl.
+  rewrite mult_comm, plus_comm.
+  rewrite mod_add. rewrite mod_small. 
+  reflexivity. apply nat_of_binary_bound.
+
+  pose (pow_of_2_pos k). omega.
+Qed.
+
+Lemma block_spec (x : bits 32) : [: block x ] = 
+  [: x ] - modulo [: x ] 32.
+Proof. unfold block. 
+  unfold block_size_mask.
+  pose (BVand_shiftl_full 27 5 x).
+  Opaque BVand vector_split. simpl in e. rewrite e. clear e.
+  pose (nat_of_binary_be_vector_append  (fst (@vector_split _ 27 5 x))
+    (@Binary.zero 5)). Opaque pow_of_2. simpl in e. rewrite e. 
+  clear e.
+  rewrite (@modulo_nat_binary 27 5).
+  generalize (@nat_of_vector_split 27 5 x). destruct @vector_split.
+  intro Hx.
+  replace [: x] with (pow_of_2 5 * [: v] + [: v0]).
+  simpl. 
+  pose (nat_of_binary_bound v).
+  pose (nat_of_binary_bound v0).
+  ring_simplify. set(foo:=pow_of_2 5 * [: v]). omega.
+Qed.
+
+Lemma instr_overlaps_block_size_spec (ip : int32) :
+  instr_overlaps_block_size ip = false -> block ip = block (next_ip ip).
+Proof.
+  funelim (instr_overlaps_block_size ip).
+  apply nat_of_binary_be_inj. 
+  rewrite ! block_spec.
+  assert([: next_ip ip] > [: ip ]). 
+
+    Unset Printing Notations. 
+    idtac.
+Set Printing 
+    rewrite e.
+    simp binary.
+    rewrite (@modulo_nat_binary 27 5).
+    symmetry.
+    assert (minx:=binary_minus_correct x (zx_be (snd (@vector_split _ 27 5 x)))).
+    do 2 red in minx.
+    replace [: snd (@vector_split _ 27 5 x)] with [: zx_be (t':=32) (snd (@vector_split _ 27 5 x)) ].
+    apply minx. clear minx.
+    funelim (binary_minus_correct x (zx_be (t':=32) (snd (@vector_split _ 27 5 x)))).
+    
+
+    repeat depelim x.
+    Opaque nat_of_binary_be. simpl.
+    simpl fst.
+    simp vector_split.
+    simpl.
+    simp vector_split.
+    unfold binary_shiftl_n_full. Opaque minus modulo_nat. simpl.
+    simpl.
+    
+
+
+  apply binary_eq_eq.
+  Print Hint binary_eq.
+  
+  
+
+instr_overlaps_block_size ip
+  with binary_plus_be (block_offset ip) (instr_length ip) :=
+  | pair offset of := negb (binary_eq (block offset) zero).
+
 
 Definition instr_is_indirect_jmp_or_call (i : instr) :=
   match i with
@@ -220,33 +306,86 @@ Definition start_addresses := list int32.
 Definition two {n} : bits (Datatypes.S (Datatypes.S n)) :=
   zx_be (Vcons true (Vcons false Vnil)).
 
-(* Equations(nocomp) build_startaddrs (ip : int32) (jtargets : regset) *)
-(*   (sa : start_addresses) *)
-(*   (icount : nat) (instrs : list instr) (p : bvec_to_nat ip < length instrs) *)
-(*   { measure (length instrs - icount) } : (regset * start_addresses) + valid_error := *)
-(*   if eq_nat_dec (Datatypes.S (bvec_to_nat ip)) (length instrs) then inl (jtargets, sa) *)
-(*   else *)
-(*     let instr := nth_prf (bvec_to_nat ip) instrs p in *)
-(*       if instr_is_disallowed instr  *)
-(*       then inr Disallowed_instruction *)
-(*       else *)
-(*         let sa := ip :: sa in *)
-(*         let jtargets := Int32Map.set ip true jtargets in *)
-(*           if instr_overlaps_block_size ip *)
-(*           then inr Block_alignment_failure *)
-(*           else if instr_is_indirect_jmp_or_call instr  *)
-(*             then if ltb icount 2  *)
-(*               then inr Bad_indirect_control *)
-(*               else if negb (binary_eq (block ip) (block (bdec (bdec ip))))  *)
-(*                 then inr Bad_indirect_control *)
-(*                 else if negb (is_nacl_jmp_idiom instr (nth_prf (bvec_to_nat (bdec ip)) instrs _))  *)
-(*                 then inr Bad_indirect_control *)
-(*                 else build_startaddrs (binc ip) jtargets sa (Datatypes.S icount) instrs _ *)
-(*             else build_startaddrs (binc ip) jtargets sa (Datatypes.S icount) instrs _. *)
-
 Section Validator.
   Variable text_limit : int32.
+
+
+  Equations(nocomp) build_startaddrs (ip : int32) (jtargets : regset) (sa : start_addresses) 
+    (prev : list instr) (instrs : list instr) : (regset * start_addresses * int32) + valid_error :=
+  build_startaddrs ip jtargets sa prev nil := inl (jtargets, sa, ip);
+  build_startaddrs ip jtargets sa prev (cons instr instrs) with instr_is_disallowed instr :=
+  | true := inr Disallowed_instruction;
+  | false with instr_overlaps_block_size ip :=
+    { | true := inr Block_alignment_failure ;
+      | false with instr_is_indirect_jmp_or_call instr :=
+        { | true with dec (ltb (List.length prev) 2) :=
+          { | left := inr Bad_indirect_control;
+            | right with negb (binary_eq (block ip) (block (bdec (bdec ip)))) :=
+              { | true := inr Bad_indirect_control;
+                | false with negb (is_nacl_jmp_idiom instr (nth_prf (bvec_to_nat (bdec ip)) instrs _)) :=
+                  { | true := inr Bad_indirect_control;
+                    | false := 
+                      let sa := ip :: sa in
+                      let jtargets := Int32Map.set ip true jtargets in
+                      let ip' := fst $ binary_plus_be ip (instr_length ip) in
+                        build_startaddrs ip' jtargets sa (instr :: prev) instrs } } 
+          } ;
+          | false := 
+            let sa := ip :: sa in
+            let jtargets := Int32Map.set ip true jtargets in
+              build_startaddrs (binc ip) jtargets sa (instr :: prev) instrs } }.
   
+  Next Obligation. admit. Defined.
+
+  Definition jtargets_inv jtargets limit :=
+    forall addr, 
+      binary_be_lt addr limit = true ->
+      BVand _ addr block_size_mask = addr -> Int32Map.get addr jtargets = true.
+
+  Lemma build_startaddrs_inv (ip : int32) (jtargets : regset) (sa : start_addresses) 
+    (prev instrs : list instr) jtargets' sas ip' :
+    build_startaddrs ip jtargets sa prev instrs = inl (jtargets', sas, ip') ->
+    jtargets_inv jtargets ip ->
+    jtargets_inv jtargets' ip'.
+  Proof.
+    funelim (build_startaddrs ip jtargets sa prev instrs).
+    specialize (H (binc ip) _ _ _ H0). apply H.
+    red; red in H1.
+    intros. 
+    rewrite Int32Map.gsspec.
+    case_eq (Int32Indexed.eq addr ip). intros.
+    subst. clear H4. reflexivity.
+    intros diffip _.
+    unfold instr_overlaps_block_size in Heq0.
+    destruct_call_eq @binary_plus_be bip. 
+    destruct o. noconf Heq0. Opaque binary_eq BVand BVxor. simpl in Heq0.
+    rewrite negb_false_iff in Heq0.
+    apply binary_eq_eq in Heq0.
+    correct bip. simpl in bip.
+    symmetry in Heq0. apply BVand_mask_zero in Heq0.
+    
+
+    Lemma BVxor_be {n} (x y z : bits n) : BVxor n x y = z ->
+      [: x ] 
+      [: x ] 
+
+
+    
+    
+
+
+    apply H with (sas). exact (binc ip). assumption.
+    clear H0.
+    red; red in H1.
+    intros. 
+    rewrite Int32Map.gsspec.
+    case_eq (Int32Indexed.eq addr ip). intros.
+    subst. clear H2. reflexivity.
+    intros.
+    apply H1. assumption.
+  Qed.
+    
+
   Program Fixpoint build_startaddrs (ip : int32) (jtargets : regset) (sa : start_addresses) 
     (prev : list instr) (instrs : list instr) { struct instrs } 
     : (regset * start_addresses) + valid_error :=
@@ -332,17 +471,42 @@ Section Validator.
             end
       end.
 
-    Definition validator (s : list instr) : unit + valid_error :=
+    Definition validator (s : list instr) : start_addresses + valid_error :=
       let jump_targets := Reg32Map.init false in
       let ip : int32 := nat_to_bvec 32 0 in
         match build_startaddrs zero jump_targets [] [] s with
           | inl (targets, sa) =>
-            direct_transfers s targets sa
+            match direct_transfers s targets sa with
+              | inl tt => inl sa
+              | inr r => inr r
+            end
           | inr r => inr r
         end.
 
 End Validator.
 
+Definition binary := list instr.
 
+Inductive exec_star : forall (l : list instr) (pc : int32) (s q : state), Prop :=
+| exec_one : forall (i : instr) (l : list instr) (pc : int32) (s q : state), 
+  exec (i, pc) s q -> exec_star (i :: l) pc s q
+| exec_next : forall (i : instr) (l : list instr) (pc : int32) (s q r : state),
+  exec (i, pc) s q -> exec_star l (stPc q) q r ->
+  exec_star (i :: l) pc s r. 
 
-    
+Definition reachable (p : list instr) (ip : int32) (ip' : int32) : Prop :=
+  forall s e : state, exec_star p ip s e -> stPc s = ip -> stPc e = ip'.
+
+Parameter text_limit : int32.
+
+Definition invariant := forall p s, validator text_limit p = inl s ->
+  forall ip, In ip s -> 
+    forall ip', reachable p ip ip' -> In ip' s.
+
+Theorem safe : invariant.
+Proof.
+  intros p s val ip ips ip' reach.
+  red in reach.  
+  induction p. unfold validator in val. simpl in val. injection val.
+  intros. subst. inversion ips.
+  
